synth, filter

src/lowparse/pulse/LowParse.Pulse.Base.fst
@@ -1,6 +1,6 @@
 module LowParse.Pulse.Base
 open FStar.Tactics.V2
-open Pulse.Lib.Pervasives
+open LowParse.Pulse.Util
 open Pulse.Lib.Slice
 open LowParse.Spec.Base
 
@@ -12,16 +12,16 @@ let serializer #k = tot_serializer #k
 let pts_to_serialized (#k: parser_kind) (#t: Type) (#p: parser k t) (s: serializer p) (input: slice byte) (#[exact (`1.0R)] pm: perm) (v: t) : vprop =
   pts_to input #pm (bare_serialize s v)
 
-let validator_success (#k: parser_kind) (#t: Type) (p: parser k t) (offset: SZ.t) (v: bytes) (off: SZ.t) : Tot prop =
-    SZ.v offset <= Seq.length v /\ (
+let validator_success (#k: parser_kind) (#t: Type) (p: parser k t) (offset: SZ.t) (v: bytes) (off: SZ.t) : GTot bool =
+    SZ.v offset <= Seq.length v && (
     let pv = parse p (Seq.slice v (SZ.v offset) (Seq.length v)) in
-    Some? pv /\
-    snd (Some?.v pv) == SZ.v off
+    Some? pv &&
+    snd (Some?.v pv) = SZ.v off
   )
 
-let validator_failure (#k: parser_kind) (#t: Type) (p: parser k t) (offset: SZ.t) (v: bytes) : Tot prop =
-    SZ.v offset <= Seq.length v /\
-    parse p (Seq.slice v (SZ.v offset) (Seq.length v)) == None
+let validator_failure (#k: parser_kind) (#t: Type) (p: parser k t) (offset: SZ.t) (v: bytes) : GTot bool =
+    SZ.v offset <= Seq.length v &&
+    None? (parse p (Seq.slice v (SZ.v offset) (Seq.length v)))
 
 inline_for_extraction
 let validator (#t: Type0) (#k: parser_kind) (p: parser k t) : Tot Type =
@@ -39,21 +39,8 @@ let validator (#t: Type0) (#k: parser_kind) (p: parser k t) : Tot Type =
     (fun x -> post x)
 
 inline_for_extraction
-```pulse
-fn validate_ext (#t: Type0) (#k1: parser_kind) (#p1: parser k1 t) (v1: validator p1) (#k2: parser_kind) (p2: parser k2 t { forall x . parse p1 x == parse p2 x }) : validator #_ #k2 p2 =
-  (input: slice byte)
-  (offset: SZ.t)
-  (#pm: perm)
-  (#v: Ghost.erased bytes)
-  (pre: vprop)
-  (t': Type0)
-  (post: (t' -> vprop))
-  (ksucc: ((off: SZ.t) -> stt t' (pts_to input #pm v ** pre ** pure (validator_success p2 offset v off)) (fun x -> post x)))
-  (kfail: (unit -> stt t' (pts_to input #pm v ** pre ** pure (validator_failure p2 offset v)) (fun x -> post x)))
-{
-  v1 input offset pre t' post ksucc kfail;
-}
-```
+let validate_ext (#t: Type0) (#k1: parser_kind) (#p1: parser k1 t) (v1: validator p1) (#k2: parser_kind) (p2: parser k2 t { forall x . parse p1 x == parse p2 x }) : validator #_ #k2 p2 =
+  v1
 
 inline_for_extraction
 ```pulse
@@ -84,6 +71,26 @@ fn validate_total_constant_size (#t: Type0) (#k: parser_kind) (p: parser k t) (s
 }
 ```
 
+let jumper_pre
+  (#t: Type0)
+  (#k: parser_kind)
+  (p: parser k t)
+  (offset: SZ.t)
+  (v: Ghost.erased bytes)
+: GTot bool
+= 
+  SZ.v offset <= Seq.length v && Some? (parse p (Seq.slice v (SZ.v offset) (Seq.length v)))  
+
+let jumper_pre'
+  (#t: Type0)
+  (#k: parser_kind)
+  (p: parser k t)
+  (offset: SZ.t)
+  (v: Ghost.erased bytes)
+: Tot prop
+= 
+  jumper_pre p offset v
+
 inline_for_extraction
 let jumper (#t: Type0) (#k: parser_kind) (p: parser k t) : Tot Type =
   (input: slice byte) ->
@@ -91,20 +98,12 @@ let jumper (#t: Type0) (#k: parser_kind) (p: parser k t) : Tot Type =
   (#pm: perm) ->
   (#v: Ghost.erased bytes) ->
   stt SZ.t
-    (pts_to input #pm v ** pure (SZ.v offset <= Seq.length v /\ Some? (parse p (Seq.slice v (SZ.v offset) (Seq.length v)))))
+    (pts_to input #pm v ** pure (jumper_pre' p offset v))
     (fun res -> pts_to input #pm v ** pure (validator_success p offset v res))
 
 inline_for_extraction
-```pulse
-fn jump_ext (#t: Type0) (#k1: parser_kind) (#p1: parser k1 t) (v1: jumper p1) (#k2: parser_kind) (p2: parser k2 t { forall x . parse p1 x == parse p2 x }) : jumper #_ #k2 p2 =
-  (input: slice byte)
-  (offset: SZ.t)
-  (#pm: perm)
-  (#v: Ghost.erased bytes)
-{
-  v1 input offset;
-}
-```
+let jump_ext (#t: Type0) (#k1: parser_kind) (#p1: parser k1 t) (v1: jumper p1) (#k2: parser_kind) (p2: parser k2 t { forall x . parse p1 x == parse p2 x }) : jumper #_ #k2 p2 =
+  v1
 
 inline_for_extraction
 ```pulse
@@ -133,7 +132,8 @@ let peek_post'
 : Tot vprop
 = exists* v1 v2 . pts_to_serialized s left #pm v1 ** pts_to right #pm v2 ** is_split input pm consumed left right ** pure (
     bare_serialize s v1 `Seq.append` v2 == v /\
-    Seq.length (bare_serialize s v1) == SZ.v consumed
+    Seq.length (bare_serialize s v1) == SZ.v consumed /\
+    parse p v == Some (v1, SZ.v consumed)
   )
 
 let peek_post
@@ -173,6 +173,64 @@ fn peek
       (s1, s2)
     }
   }
+}
+```
+
+let peek_stick_post'
+  (#k: parser_kind) (#t: Type) (#p: parser k t) (s: serializer p)
+  (input: slice byte)
+  (pm: perm)
+  (v: bytes)
+  (consumed: SZ.t)
+  (left right: slice byte)
+: Tot vprop
+= exists* v1 v2 . pts_to_serialized s left #pm v1 ** pts_to right #pm v2 ** ((pts_to_serialized s left #pm v1 ** pts_to right #pm v2) @==> pts_to input #pm v) ** pure (
+    bare_serialize s v1 `Seq.append` v2 == v /\
+    Seq.length (bare_serialize s v1) == SZ.v consumed /\
+    parse p v == Some (v1, SZ.v consumed)
+  )
+
+let peek_stick_post
+  (#k: parser_kind) (#t: Type) (#p: parser k t) (s: serializer p)
+  (input: slice byte)
+  (pm: perm)
+  (v: bytes)
+  (consumed: SZ.t)
+  (res: (slice byte & slice byte))
+: Tot vprop
+= let (left, right) = res in
+  peek_stick_post' s input pm v consumed left right
+
+```pulse
+fn peek_stick
+  (#t: Type0) (#k: parser_kind) (#p: parser k t) (s: serializer p)
+  (input: slice byte)
+  (#pm: perm)
+  (#v: Ghost.erased bytes)
+  (consumed: SZ.t)
+  requires (pts_to input #pm v ** pure (validator_success #k #t p 0sz v (consumed)))
+  returns res: (slice byte & slice byte)
+  ensures peek_stick_post s input pm v consumed res
+{
+  let res = peek s input consumed;
+  match res { Mktuple2 left right -> {
+    unfold (peek_post s input pm v consumed res);
+    unfold (peek_post' s input pm v consumed left right);
+    with v1 v2 . assert (pts_to_serialized s left #pm v1 ** pts_to right #pm v2);
+    ghost
+    fn aux
+      (_foo: unit)
+      requires (is_split input pm consumed left right ** (pts_to_serialized s left #pm v1 ** pts_to right #pm v2))
+      ensures pts_to input #pm v
+      {
+        unfold (pts_to_serialized s left #pm v1);
+        join left right input
+      };
+    intro_stick (pts_to_serialized s left #pm v1 ** pts_to right #pm v2) (pts_to input #pm v) (is_split input pm consumed left right) aux;
+    fold (peek_stick_post' s input pm v consumed left right);
+    fold (peek_stick_post s input pm v consumed (left, right));
+    (left, right)
+  }}
 }
 ```
 
